src/Utility.v
@@ -11,7 +11,7 @@ Local Open Scope Z_scope.
    no matter whether it's a 32-bit or 64-bit machine. *)
 Definition MachineInt := Z.
 
-Class MachineWidth(t: Set) := mkMachineWidth {
+Class MachineWidth(t: Type) := mkMachineWidth {
   (* arithmetic operations (inherited from Integral in Haskell) *)
   add: t -> t -> t;
   sub: t -> t -> t;
@@ -123,7 +123,7 @@ Notation fromImm := (@ZToReg _ _) (only parsing).
 
 Section Derived.
 
-  Context {t: Set}.
+  Context {t: Type}.
   Context {MW: MachineWidth t}.
 
   Definition XLEN_in_bytes: Z := XLEN / 8.
