src/MinimalLogging.v
@@ -12,11 +12,11 @@ Require Import riscv.Minimal.
 
 Section Riscv.
 
-  Context {t: Set}.
+  Context {t: Type}.
 
   Context {MW: MachineWidth t}.
 
-  Context {Mem: Set}.
+  Context {Mem: Type}.
 
   Context {MemIsMem: Memory Mem t}.
 
